Translation/ITypingMore.v
@@ -1,0 +1,878 @@
+From Coq Require Import Bool String List BinPos Compare_dec Omega.
+From Equations Require Import Equations DepElimDec.
+From Template Require Import Ast utils Typing.
+From Translation Require Import SAst SLiftSubst SCommon ITyping ITypingLemmata.
+
+(* We state several inversion lemmata on a by need basis. *)
+
+Lemma inversionRel :
+  forall {Σ Γ n T},
+    type_glob Σ ->
+    Σ ;;; Γ |-i sRel n : T ->
+    ∑ isdecl s,
+      let A := lift0 (S n) (safe_nth Γ (exist _ n isdecl)).(sdecl_type) in
+      Σ ;;; Γ |-i A = T : sSort s.
+Proof.
+  intros Σ Γ n T hg h. dependent induction h.
+  - exists isdecl.
+    assert (Σ ;;; Γ |-i sRel n : lift0 (S n) (safe_nth Γ (exist _ n isdecl)).(sdecl_type)) by (now constructor).
+    destruct (istype_type hg X) as [s hs].
+    exists s. apply eq_reflexivity. eassumption.
+  - destruct (IHh1 hg) as [isdecl [s' h]].
+    exists isdecl, s'.
+    eapply eq_transitivity.
+    + exact h.
+    + destruct (eq_typing hg e) as [hAs _].
+      destruct (eq_typing hg h) as [_ hAs'].
+      destruct (uniqueness hAs hAs') as [? ?].
+      eapply eq_conv ; eassumption.
+Defined.
+
+Lemma inversionSort :
+  forall {Σ Γ s T},
+    type_glob Σ ->
+    Σ ;;; Γ |-i sSort s : T ->
+    Σ ;;; Γ |-i sSort (succ_sort s) = T : sSort (succ_sort (succ_sort s)).
+Proof.
+  intros Σ Γ s T hg h.
+  dependent induction h.
+
+  - apply eq_reflexivity. apply type_Sort. assumption.
+
+  - specialize (IHh1 hg).
+    eapply eq_transitivity.
+    + eassumption.
+    + destruct (eq_typing hg e) as [hAs0 _].
+      destruct (eq_typing hg IHh1) as [_ hAss].
+      destruct (uniqueness hAs0 hAss) as [? ?].
+      eapply eq_conv ; eassumption.
+Defined.
+
+Lemma inversionInd :
+  forall {Σ Γ ind T},
+    type_glob Σ ->
+    Σ ;;; Γ |-i sInd ind : T ->
+    ∑ univs decl (isdecl : sdeclared_inductive (fst Σ) ind univs decl) s,
+      Σ ;;; Γ |-i decl.(sind_type) = T : sSort s.
+Proof.
+  intros Σ Γ ind T hg h.
+  dependent induction h.
+
+  - exists univs, decl, isdecl.
+    destruct (typed_ind_type hg isdecl) as [s h]. exists s.
+    apply eq_reflexivity.
+    change (sSort s) with (lift #|Γ| #|@nil scontext_decl| (sSort s)).
+    replace (sind_type decl)
+      with (lift #|Γ| #|@nil scontext_decl| (sind_type decl))
+      by (erewrite lift_ind_type by eassumption ; reflexivity).
+    eapply meta_ctx_conv.
+    + eapply @type_lift with (Γ := []) (Ξ := []) (Δ := Γ).
+      * assumption.
+      * assumption.
+      * rewrite nil_cat. assumption.
+    + cbn. apply nil_cat.
+
+  - destruct (IHh1 hg) as [univs [decl [isdecl [s' eq]]]].
+    exists univs, decl, isdecl, s'.
+    eapply eq_transitivity.
+    + eassumption.
+    + destruct (eq_typing hg e) as [hAs _].
+      destruct (eq_typing hg eq) as [_ hAss0].
+      destruct (uniqueness hAs hAss0) as [? ?].
+      eapply eq_conv ; eassumption.
+Defined.
+
+Lemma inversionProd :
+  forall {Σ Γ n A B T},
+    type_glob Σ ->
+    Σ ;;; Γ |-i sProd n A B : T ->
+    ∑ s1 s2,
+      (Σ ;;; Γ |-i A : sSort s1) *
+      (Σ ;;; Γ ,, svass n A |-i B : sSort s2) *
+      (Σ ;;; Γ |-i sSort (max_sort s1 s2) = T : sSort (succ_sort (max_sort s1 s2))).
+Proof.
+  intros Σ Γ n A B T hg h.
+  dependent induction h.
+
+  - exists s1, s2. repeat split.
+    + assumption.
+    + assumption.
+    + apply eq_reflexivity. apply type_Sort. apply (typing_wf h1).
+
+  - destruct (IHh1 hg) as [s1 [s2 [[? ?] ?]]].
+    exists s1, s2. repeat split.
+    + assumption.
+    + assumption.
+    + eapply eq_transitivity.
+      * eassumption.
+      * destruct (eq_typing hg e) as [hAs _].
+        destruct (eq_typing hg pi2_0) as [_ hAsm].
+        destruct (uniqueness hAs hAsm).
+        eapply eq_conv ; eassumption.
+Defined.
+
+Lemma inversionLambda :
+  forall {Σ Γ na A B t T},
+    type_glob Σ ->
+    Σ ;;; Γ |-i sLambda na A B t : T ->
+      ∑ s1 s2,
+        (Σ ;;; Γ |-i A : sSort s1) *
+        (Σ ;;; Γ ,, svass na A |-i B : sSort s2) *
+        (Σ ;;; Γ ,, svass na A |-i t : B) *
+        (Σ ;;; Γ |-i sProd na A B = T : sSort (max_sort s1 s2)).
+Proof.
+  intros Σ Γ na A B t T hg h.
+  dependent induction h.
+
+  - exists s1, s2. repeat split ; try eassumption.
+    apply cong_Prod.
+    all: apply eq_reflexivity ; assumption.
+
+  - destruct (IHh1 hg) as [s1 [s2 [[[? ?] ?] ?]]].
+    exists s1, s2. repeat split.
+    all: try assumption.
+    eapply eq_transitivity.
+    + eassumption.
+    + destruct (eq_typing hg e) as [i1 _].
+      destruct (eq_typing hg pi2_1) as [_ i2].
+      destruct (uniqueness i1 i2).
+      eapply eq_conv ; eassumption.
+Defined.
+
+Lemma inversionApp :
+  forall {Σ Γ t n A B u T},
+    type_glob Σ ->
+    Σ ;;; Γ |-i sApp t n A B u : T ->
+    ∑ s1 s2,
+      (Σ ;;; Γ |-i A : sSort s1) *
+      (Σ ;;; Γ ,, svass n A |-i B : sSort s2) *
+      (Σ ;;; Γ |-i t : sProd n A B) *
+      (Σ ;;; Γ |-i u : A) *
+      (Σ ;;; Γ |-i B{ 0 := u } = T : sSort s2).
+Proof.
+  intros Σ Γ t n A B u T hg H.
+  dependent induction H.
+
+  - exists s1, s2.
+    repeat split ; try easy.
+    apply eq_reflexivity.
+    change (sSort s2) with ((sSort s2){0 := u}).
+    eapply typing_subst ; eassumption.
+
+  - destruct (IHtyping1 hg) as [s1 [s2 [[[[? ?] ?] ?] ?]]].
+    exists s1, s2. repeat split ; try easy.
+    eapply eq_transitivity.
+    + eassumption.
+    + destruct (eq_typing hg e) as [hAs _].
+      destruct (eq_typing hg pi2_2) as [_ hAs2].
+      destruct (uniqueness hAs hAs2).
+      eapply eq_conv ; eassumption.
+Defined.
+
+Lemma inversionEq :
+  forall {Σ Γ A u v T},
+    type_glob Σ ->
+    Σ ;;; Γ |-i sEq A u v : T ->
+    ∑ s,
+      (Σ ;;; Γ |-i A : sSort s) *
+      (Σ ;;; Γ |-i u : A) *
+      (Σ ;;; Γ |-i v : A) *
+      (Σ ;;; Γ |-i sSort s = T : sSort (succ_sort s)).
+Proof.
+  intros Σ Γ A u v T hg h.
+  dependent induction h.
+  - exists s. repeat split ; try easy.
+    eapply eq_reflexivity. apply type_Sort.
+    apply (typing_wf h1).
+  - destruct (IHh1 hg) as [s' [[[hA hu] hv] heq]].
+    exists s'. repeat split ; try easy.
+    eapply eq_transitivity.
+    + exact heq.
+    + destruct (eq_typing hg heq) as [_ hA01].
+      destruct (eq_typing hg e) as [hA02 _].
+      destruct (uniqueness hA02 hA01) as [s'' h''].
+      eapply eq_conv ; eassumption.
+Defined.
+
+Lemma inversionRefl :
+  forall {Σ Γ A u T},
+    type_glob Σ ->
+    Σ ;;; Γ |-i sRefl A u : T ->
+    ∑ s,
+      (Σ ;;; Γ |-i A : sSort s) *
+      (Σ ;;; Γ |-i u : A) *
+      (Σ ;;; Γ |-i sEq A u u = T : sSort s).
+Proof.
+  intros Σ Γ A u T hg h.
+  dependent induction h.
+
+  - exists s. repeat split ; try easy.
+    apply eq_reflexivity. apply type_Eq ; assumption.
+
+  - destruct (IHh1 hg) as [s' [[hA hu] eq]].
+    exists s'. repeat split ; try easy.
+    destruct (eq_typing hg e) as [i1 _].
+    destruct (eq_typing hg eq) as [_ i2].
+    destruct (uniqueness i1 i2).
+    eapply eq_transitivity.
+    + eassumption.
+    + eapply eq_conv ; eassumption.
+Defined.
+
+Lemma inversionJ :
+  forall {Σ Γ A u P w v p T},
+    type_glob Σ ->
+    Σ ;;; Γ |-i sJ A u P w v p : T ->
+    ∑ s1 s2 nx ne,
+      (Σ ;;; Γ |-i A : sSort s1) *
+      (Σ ;;; Γ |-i u : A) *
+      (Σ ;;; Γ |-i v : A) *
+      (Σ ;;; Γ ,, svass nx A ,,
+         svass ne (sEq (lift0 1 A) (lift0 1 u) (sRel 0)) |-i P : sSort s2) *
+      (Σ ;;; Γ |-i p : sEq A u v) *
+      (Σ ;;; Γ |-i w : (P {1 := u}){0 := sRefl A u}) *
+      (Σ ;;; Γ |-i P{1 := v}{0 := p} = T : sSort s2).
+Proof.
+  intros Σ Γ A u P w v p T hg H.
+  dependent induction H.
+
+  - exists s1, s2, nx, ne. repeat split ; try easy.
+    apply eq_reflexivity.
+    change (sSort s2) with ((sSort s2){1 := v}{0 := p}).
+    eapply typing_subst2.
+    + assumption.
+    + eassumption.
+    + assumption.
+    + cbn. rewrite !lift_subst, lift00.
+      assumption.
+
+  - destruct (IHtyping1 hg)
+      as [s1 [s2 [nx [ne [[[[[[? ?] ?] ?] ?] ?] ?]]]]].
+    exists s1, s2, nx, ne. repeat split ; try easy.
+    eapply eq_transitivity.
+    + eassumption.
+    + destruct (eq_typing hg e) as [hAs _].
+      destruct (eq_typing hg pi2_4) as [_ hAs2].
+      destruct (uniqueness hAs hAs2).
+      eapply eq_conv ; eassumption.
+Defined.
+
+Lemma inversionTransport :
+  forall {Σ Γ A B p t T},
+    type_glob Σ ->
+    Σ ;;; Γ |-i sTransport A B p t : T ->
+    ∑ s,
+      (Σ ;;; Γ |-i p : sEq (sSort s) A B) *
+      (Σ ;;; Γ |-i t : A) *
+      (Σ ;;; Γ |-i A : sSort s) *
+      (Σ ;;; Γ |-i B : sSort s) *
+      (Σ ;;; Γ |-i B = T : sSort s).
+Proof.
+  intros Σ Γ A B p t T hg h.
+  dependent induction h.
+
+  - exists s. repeat split ; try easy.
+    apply eq_reflexivity. assumption.
+
+  - destruct (IHh1 hg) as [s' [[[[? ?] ?] ?] ?]].
+    exists s'. repeat split ; try easy.
+    eapply eq_transitivity.
+    + eassumption.
+    + destruct (eq_typing hg e) as [hA1 _].
+      destruct (eq_typing hg pi2_2) as [_ hA2].
+      destruct (uniqueness hA1 hA2).
+      eapply eq_conv ; eassumption.
+Defined.
+
+Lemma inversionHeq :
+  forall {Σ Γ A B a b T},
+    type_glob Σ ->
+    Σ ;;; Γ |-i sHeq A a B b : T ->
+    ∑ s,
+      (Σ ;;; Γ |-i A : sSort s) *
+      (Σ ;;; Γ |-i B : sSort s) *
+      (Σ ;;; Γ |-i a : A) *
+      (Σ ;;; Γ |-i b : B) *
+      (Σ ;;; Γ |-i sSort (succ_sort s) = T : sSort (succ_sort (succ_sort s))).
+Proof.
+  intros Σ Γ A B a b T hg h.
+  dependent induction h.
+
+  - exists s. repeat split ; try easy.
+    apply eq_reflexivity. apply type_Sort. apply (typing_wf h1).
+
+  - destruct (IHh1 hg) as [s' [[[[? ?] ?] ?] ?]].
+    exists s'. repeat split ; try easy.
+    eapply eq_transitivity.
+    + eassumption.
+    + destruct (eq_typing hg e) as [i1 _].
+      destruct (eq_typing hg pi2_2) as [_ i2].
+      destruct (uniqueness i1 i2).
+      eapply eq_conv ; eassumption.
+Defined.
+
+Lemma inversionPack :
+  forall {Σ Γ A1 A2 T},
+    type_glob Σ ->
+    Σ ;;; Γ |-i sPack A1 A2 : T ->
+    ∑ s,
+      (Σ ;;; Γ |-i A1 : sSort s) *
+      (Σ ;;; Γ |-i A2 : sSort s) *
+      (Σ ;;; Γ |-i sSort s = T : sSort (succ_sort s)).
+Proof.
+  intros Σ Γ A1 A2 T hg h.
+  dependent induction h.
+
+  - exists s. repeat split ; try easy.
+    apply eq_reflexivity. apply type_Sort. apply (typing_wf h1).
+
+  - destruct (IHh1 hg) as [s' [[? ?] ?]].
+    exists s'. repeat split ; try easy.
+    eapply eq_transitivity.
+    + eassumption.
+    + destruct (eq_typing hg e) as [i1 _].
+      destruct (eq_typing hg pi2_0) as [_ i2].
+      destruct (uniqueness i1 i2).
+      eapply eq_conv ; eassumption.
+Defined.
+
+(* We state some admissible typing rules *)
+Lemma type_conv' :
+  forall {Σ Γ t A B s},
+    type_glob Σ ->
+    Σ ;;; Γ |-i t : A ->
+    Σ ;;; Γ |-i A = B : sSort s ->
+    Σ ;;; Γ |-i t : B.
+Proof.
+  intros Σ Γ t A B s hg ht eq.
+  eapply type_conv.
+  - eassumption.
+  - apply (eq_typing hg eq).
+  - assumption.
+Defined.
+
+Lemma heq_sort :
+  forall {Σ Γ s1 s2 A B p},
+    type_glob Σ ->
+    Σ ;;; Γ |-i p : sHeq (sSort s1) A (sSort s2) B ->
+    Σ ;;; Γ |-i p : sHeq (sSort s1) A (sSort s1) B.
+Proof.
+  intros Σ Γ s1 s2 A B p hg h.
+  destruct (istype_type hg h) as [? i].
+  destruct (inversionHeq hg i) as [? [[[[e1 e2] ?] ?] ?]].
+  pose proof (sorts_in_sort e2 e1) as eq.
+  eapply type_conv'.
+  - assumption.
+  - eassumption.
+  - apply cong_Heq.
+    all: try (apply eq_reflexivity ; eassumption).
+    assumption.
+Defined.
+
+Lemma type_HeqToEq' :
+  forall {Σ Γ A u v p},
+    type_glob Σ ->
+    Σ ;;; Γ |-i p : sHeq A u A v ->
+    Σ ;;; Γ |-i sHeqToEq p : sEq A u v.
+Proof.
+  intros Σ Γ A u v p hg h.
+  destruct (istype_type hg h) as [? i].
+  destruct (inversionHeq hg i) as [? [[[[? ?] ?] ?] ?]].
+  eapply type_HeqToEq ; eassumption.
+Defined.
+
+Fact sort_heq :
+  forall {Σ Γ s1 s2 A B e},
+    type_glob Σ ->
+    Σ ;;; Γ |-i e : sHeq (sSort s1) A (sSort s2) B ->
+    Σ ;;; Γ |-i sHeqToEq e : sEq (sSort s1) A B.
+Proof.
+  intros Σ Γ s1 s2 A B e hg h.
+  destruct (istype_type hg h) as [? hty].
+  destruct (inversionHeq hg hty) as [? [[[[? ?] ?] ?] ?]].
+  eapply type_HeqToEq' ; try assumption.
+  eapply heq_sort ; eassumption.
+Defined.
+
+Corollary sort_heq_ex :
+  forall {Σ Γ s1 s2 A B e},
+    type_glob Σ ->
+    Σ ;;; Γ |-i e : sHeq (sSort s1) A (sSort s2) B ->
+    ∑ p, Σ ;;; Γ |-i p : sEq (sSort s1) A B.
+Proof.
+  intros Σ Γ s A B e hg h.
+  eexists. now eapply sort_heq.
+Defined.
+
+Lemma type_HeqRefl' :
+  forall {Σ Γ A a},
+    type_glob Σ ->
+    Σ ;;; Γ |-i a : A ->
+    Σ ;;; Γ |-i sHeqRefl A a : sHeq A a A a.
+Proof.
+  intros Σ Γ A a hg h.
+  destruct (istype_type hg h).
+  eapply type_HeqRefl ; eassumption.
+Defined.
+
+Lemma type_HeqSym' :
+  forall {Σ Γ A a B b p},
+    type_glob Σ ->
+    Σ ;;; Γ |-i p : sHeq A a B b ->
+    Σ ;;; Γ |-i sHeqSym p : sHeq B b A a.
+Proof.
+  intros Σ Γ A a B b p hg h.
+  destruct (istype_type hg h) as [? hty].
+  destruct (inversionHeq hg hty) as [? [[[[? ?] ?] ?] ?]].
+  now eapply type_HeqSym.
+Defined.
+
+Lemma type_HeqTrans' :
+  forall {Σ Γ A a B b C c p q},
+    type_glob Σ ->
+    Σ ;;; Γ |-i p : sHeq A a B b ->
+    Σ ;;; Γ |-i q : sHeq B b C c ->
+    Σ ;;; Γ |-i sHeqTrans p q : sHeq A a C c.
+Proof.
+  intros Σ Γ A a B b C c p q hg h1 h2.
+  destruct (istype_type hg h1) as [? i1].
+  destruct (inversionHeq hg i1) as [? [[[[? iB1] ?] ?] ?]].
+  destruct (istype_type hg h2) as [? i2].
+  destruct (inversionHeq hg i2) as [? [[[[iB2 ?] ?] ?] ?]].
+  eapply type_HeqTrans. all: try eassumption.
+  destruct (uniqueness iB2 iB1) as [? eq].
+  eapply type_conv ; [ eassumption | idtac | eassumption ].
+  apply (eq_typing hg eq).
+Defined.
+
+Lemma type_HeqTransport' :
+  forall {Σ Γ s A B p t},
+    type_glob Σ ->
+    Σ ;;; Γ |-i t : A ->
+    Σ ;;; Γ |-i p : sEq (sSort s) A B ->
+    Σ ;;; Γ |-i sHeqTransport p t : sHeq A t B (sTransport A B p t).
+Proof.
+  intros Σ Γ s A B p t hg ht hp.
+  destruct (istype_type hg hp) as [? i].
+  destruct (inversionEq hg i) as [? [[[? ?] ?] ?]].
+  eapply type_HeqTransport ; eassumption.
+Defined.
+
+Lemma type_CongProd'' :
+  forall {Σ Γ s z nx ny np A1 A2 B1 B2 pA pB},
+    type_glob Σ ->
+    Σ ;;; Γ |-i pA : sHeq (sSort s) A1 (sSort s) A2 ->
+    Σ ;;; Γ ,, svass np (sPack A1 A2)
+    |-i pB : sHeq (sSort z) ((lift 1 1 B1){ 0 := sProjT1 (sRel 0) })
+                (sSort z) ((lift 1 1 B2){ 0 := sProjT2 (sRel 0) }) ->
+    Σ ;;; Γ ,, svass nx A1 |-i B1 : sSort z ->
+    Σ ;;; Γ ,, svass ny A2 |-i B2 : sSort z ->
+    Σ ;;; Γ |-i sCongProd B1 B2 pA pB :
+    sHeq (sSort (max_sort s z)) (sProd nx A1 B1)
+         (sSort (max_sort s z)) (sProd ny A2 B2).
+Proof.
+  intros Σ Γ s z nx ny np A1 A2 B1 B2 pA pB hg hpA hpB hB1 hB2.
+  destruct (istype_type hg hpA) as [? ipA].
+  destruct (inversionHeq hg ipA) as [? [[[[? ?] ?] ?] ?]].
+  destruct (istype_type hg hpB) as [? ipB].
+  destruct (inversionHeq hg ipB) as [? [[[[? ?] ?] ?] ?]].
+  eapply type_CongProd.
+  all: eassumption.
+Defined.
+
+Lemma prod_sorts :
+  forall {Σ Γ s1 s2 z1 z2 nx ny np A1 A2 B1 B2 pA pB},
+    type_glob Σ ->
+    Σ ;;; Γ |-i pA : sHeq (sSort s1) A1 (sSort s2) A2 ->
+    Σ ;;; Γ ,, svass np (sPack A1 A2)
+    |-i pB : sHeq (sSort z1) ((lift 1 1 B1){ 0 := sProjT1 (sRel 0) })
+                (sSort z2) ((lift 1 1 B2){ 0 := sProjT2 (sRel 0) }) ->
+    Σ ;;; Γ ,, svass nx A1 |-i B1 : sSort z1 ->
+    Σ ;;; Γ ,, svass ny A2 |-i B2 : sSort z2 ->
+    ∑ ss zz mm,
+      (Σ ;;; Γ |-i sSort s1 = sSort s2 : sSort ss) *
+      (Σ ;;; Γ ,, svass ny A2 |-i sSort z2 = sSort z1 : sSort zz) *
+      (Σ ;;; Γ |-i sSort (max_sort s1 z1) = sSort (max_sort s2 z2) : sSort mm).
+Proof.
+  intros Σ Γ s1 s2 z1 z2 nx ny np A1 A2 B1 B2 pA pB hg hpA hpB hB1 hB2.
+  assert (hs : ∑ ss, Σ ;;; Γ |-i sSort s1 = sSort s2 : sSort ss).
+  { destruct (istype_type hg hpA) as [? ipA].
+    destruct (inversionHeq hg ipA) as [? [[[[e1 e2] ?] ?] ?]].
+    pose proof (sorts_in_sort e1 e2).
+    eexists. eassumption.
+  }
+  destruct hs as [ss hss]. exists ss.
+  assert (hz : ∑ zz, Σ;;; Γ,, svass ny A2 |-i sSort z2 = sSort z1 : sSort zz).
+  { destruct (istype_type hg hpB) as [? ipB].
+    destruct (inversionHeq hg ipB) as [? [[[[f1 f2] ?] ?] ?]].
+    pose proof (sorts_in_sort f2 f1).
+    eexists. eapply strengthen_sort_eq.
+    - eassumption.
+    - eapply typing_wf. eassumption.
+  }
+  destruct hz as [zz hzz]. exists zz.
+  assert (hP1 : Σ ;;; Γ |-i sProd nx A1 B1 : sSort (max_sort s1 z1)).
+  { destruct (istype_type hg hpA) as [? ipA].
+    destruct (inversionHeq hg ipA) as [? [[[[e1 e2] ?] ?] ?]].
+    apply type_Prod ; eassumption.
+  }
+  assert (hP2 : Σ ;;; Γ |-i sProd nx A1 B1 : sSort (max_sort s2 z2)).
+  { destruct (istype_type hg hpA) as [? ipA].
+    destruct (inversionHeq hg ipA) as [? [[[[e1 e2] ?] ?] ?]].
+    apply type_Prod.
+    - eapply type_conv' ; eassumption.
+    - eapply type_conv'.
+      + assumption.
+      + eassumption.
+      + apply eq_symmetry.
+        eapply strengthen_sort_eq.
+        * eassumption.
+        * eapply typing_wf. eassumption.
+  }
+  destruct (uniqueness hP1 hP2) as [mm hmm]. exists mm.
+  repeat split.
+  - assumption.
+  - assumption.
+  - assumption.
+Defined.
+
+Lemma type_CongProd' :
+  forall {Σ Γ s1 s2 z1 z2 nx ny np A1 A2 B1 B2 pA pB},
+    type_glob Σ ->
+    Σ ;;; Γ |-i pA : sHeq (sSort s1) A1 (sSort s2) A2 ->
+    Σ ;;; Γ ,, svass np (sPack A1 A2)
+    |-i pB : sHeq (sSort z1) ((lift 1 1 B1){ 0 := sProjT1 (sRel 0) })
+                (sSort z2) ((lift 1 1 B2){ 0 := sProjT2 (sRel 0) }) ->
+    Σ ;;; Γ ,, svass nx A1 |-i B1 : sSort z1 ->
+    Σ ;;; Γ ,, svass ny A2 |-i B2 : sSort z2 ->
+    Σ ;;; Γ |-i sCongProd B1 B2 pA pB :
+    sHeq (sSort (max_sort s1 z1)) (sProd nx A1 B1)
+         (sSort (max_sort s2 z2)) (sProd ny A2 B2).
+Proof.
+  intros Σ Γ s1 s2 z1 z2 nx ny np A1 A2 B1 B2 pA pB hg hpA hpB hB1 hB2.
+  destruct (prod_sorts hg hpA hpB hB1 hB2) as [ss [zz [mm [[e e0] e1]]]].
+  eapply type_conv'.
+  - assumption.
+  - eapply type_CongProd''.
+    + assumption.
+    + eapply heq_sort ; eassumption.
+    + eapply heq_sort ; eassumption.
+    + eassumption.
+    + eapply type_conv'.
+      * assumption.
+      * eassumption.
+      * eassumption.
+  - apply cong_Heq.
+    all: try apply eq_reflexivity.
+    + apply type_Sort. eapply typing_wf. eassumption.
+    + eapply eq_conv.
+      * eassumption.
+      * eapply eq_symmetry. eapply inversionSort ; try assumption.
+        apply (eq_typing hg e1).
+    + destruct (istype_type hg hpA) as [? ipA].
+      destruct (inversionHeq hg ipA) as [? [[[[? ?] ?] ?] ?]].
+      apply type_Prod ; eassumption.
+    + destruct (istype_type hg hpA) as [? ipA].
+      destruct (inversionHeq hg ipA) as [? [[[[? ?] ?] ?] ?]].
+      apply type_Prod.
+      * eapply type_conv'.
+        -- assumption.
+        -- eassumption.
+        -- eapply eq_symmetry. eassumption.
+      * eapply type_conv' ; eassumption.
+Defined.
+
+Lemma type_CongLambda'' :
+  forall {Σ Γ s z nx ny np A1 A2 B1 B2 t1 t2 pA pB pt},
+    type_glob Σ ->
+    Σ ;;; Γ |-i pA : sHeq (sSort s) A1 (sSort s) A2 ->
+    Σ ;;; Γ ,, svass np (sPack A1 A2)
+    |-i pB : sHeq (sSort z) ((lift 1 1 B1){ 0 := sProjT1 (sRel 0) })
+                 (sSort z) ((lift 1 1 B2){ 0 := sProjT2 (sRel 0) }) ->
+    Σ ;;; Γ ,, svass np (sPack A1 A2)
+    |-i pt : sHeq ((lift 1 1 B1){ 0 := sProjT1 (sRel 0) })
+                 ((lift 1 1 t1){ 0 := sProjT1 (sRel 0) })
+                 ((lift 1 1 B2){ 0 := sProjT2 (sRel 0) })
+                 ((lift 1 1 t2){ 0 := sProjT2 (sRel 0) }) ->
+    Σ ;;; Γ ,, svass nx A1 |-i B1 : sSort z ->
+    Σ ;;; Γ ,, svass ny A2 |-i B2 : sSort z ->
+    Σ ;;; Γ ,, svass nx A1 |-i t1 : B1 ->
+    Σ ;;; Γ ,, svass ny A2 |-i t2 : B2 ->
+    Σ ;;; Γ |-i sCongLambda B1 B2 t1 t2 pA pB pt :
+               sHeq (sProd nx A1 B1) (sLambda nx A1 B1 t1)
+                    (sProd ny A2 B2) (sLambda ny A2 B2 t2).
+Proof.
+  intros Σ Γ s z nx ny np A1 A2 B1 B2 t1 t2 pA pB pt
+         hg hpA hpB hpt hB1 hB2 ht1 ht2.
+  destruct (istype_type hg hpA) as [? ipA].
+  destruct (inversionHeq hg ipA) as [? [[[[? ?] ?] ?] ?]].
+  destruct (istype_type hg hpB) as [? ipB].
+  destruct (inversionHeq hg ipB) as [? [[[[? ?] ?] ?] ?]].
+  destruct (istype_type hg hpt) as [? ipt].
+  destruct (inversionHeq hg ipt) as [? [[[[? ?] ?] ?] ?]].
+  eapply type_CongLambda ; eassumption.
+Defined.
+
+Lemma type_CongLambda' :
+  forall {Σ Γ s1 s2 z1 z2 nx ny np A1 A2 B1 B2 t1 t2 pA pB pt},
+    type_glob Σ ->
+    Σ ;;; Γ |-i pA : sHeq (sSort s1) A1 (sSort s2) A2 ->
+    Σ ;;; Γ ,, svass np (sPack A1 A2)
+    |-i pB : sHeq (sSort z1) ((lift 1 1 B1){ 0 := sProjT1 (sRel 0) })
+                 (sSort z2) ((lift 1 1 B2){ 0 := sProjT2 (sRel 0) }) ->
+    Σ ;;; Γ ,, svass np (sPack A1 A2)
+    |-i pt : sHeq ((lift 1 1 B1){ 0 := sProjT1 (sRel 0) })
+                 ((lift 1 1 t1){ 0 := sProjT1 (sRel 0) })
+                 ((lift 1 1 B2){ 0 := sProjT2 (sRel 0) })
+                 ((lift 1 1 t2){ 0 := sProjT2 (sRel 0) }) ->
+    Σ ;;; Γ ,, svass nx A1 |-i B1 : sSort z1 ->
+    Σ ;;; Γ ,, svass ny A2 |-i B2 : sSort z2 ->
+    Σ ;;; Γ ,, svass nx A1 |-i t1 : B1 ->
+    Σ ;;; Γ ,, svass ny A2 |-i t2 : B2 ->
+    Σ ;;; Γ |-i sCongLambda B1 B2 t1 t2 pA pB pt :
+               sHeq (sProd nx A1 B1) (sLambda nx A1 B1 t1)
+                    (sProd ny A2 B2) (sLambda ny A2 B2 t2).
+Proof.
+  intros Σ Γ s1 s2 z1 z2 nx ny np A1 A2 B1 B2 t1 t2 pA pB pt hg
+         hpA hpB hpt hB1 hB2 ht1 ht2.
+  destruct (prod_sorts hg hpA hpB hB1 hB2) as [ss [zz [mm [[e e0] e1]]]].
+  eapply type_CongLambda''.
+  - assumption.
+  - eapply heq_sort ; eassumption.
+  - eapply heq_sort ; eassumption.
+  - eassumption.
+  - assumption.
+  - eapply type_conv' ; eassumption.
+  - assumption.
+  - assumption.
+Defined.
+
+Lemma type_CongApp'' :
+  forall {Σ Γ s z nx ny np A1 A2 B1 B2 u1 u2 v1 v2 pA pB pu pv},
+    type_glob Σ ->
+    Σ ;;; Γ |-i pA : sHeq (sSort s) A1 (sSort s) A2 ->
+    Σ ;;; Γ ,, svass np (sPack A1 A2)
+    |-i pB : sHeq (sSort z) ((lift 1 1 B1){ 0 := sProjT1 (sRel 0) })
+                 (sSort z) ((lift 1 1 B2){ 0 := sProjT2 (sRel 0) }) ->
+    Σ ;;; Γ |-i pu : sHeq (sProd nx A1 B1) u1 (sProd ny A2 B2) u2 ->
+    Σ ;;; Γ |-i pv : sHeq A1 v1 A2 v2 ->
+    Σ ;;; Γ ,, svass nx A1 |-i B1 : sSort z ->
+    Σ ;;; Γ ,, svass ny A2 |-i B2 : sSort z ->
+    Σ ;;; Γ |-i sCongApp B1 B2 pu pA pB pv :
+               sHeq (B1{0 := v1}) (sApp u1 nx A1 B1 v1)
+                    (B2{0 := v2}) (sApp u2 ny A2 B2 v2).
+Proof.
+  intros Σ Γ s z nx ny np A1 A2 B1 B2 u1 u2 v1 v2 pA pB pu pv
+         hg hpA hpB hpu hpv hB1 hB2.
+  destruct (istype_type hg hpA) as [? ipA].
+  destruct (inversionHeq hg ipA) as [? [[[[? ?] ?] ?] ?]].
+  destruct (istype_type hg hpB) as [? ipB].
+  destruct (inversionHeq hg ipB) as [? [[[[? ?] ?] ?] ?]].
+  destruct (istype_type hg hpu) as [? ipu].
+  destruct (inversionHeq hg ipu) as [? [[[[? ?] ?] ?] ?]].
+  destruct (istype_type hg hpv) as [? ipv].
+  destruct (inversionHeq hg ipv) as [? [[[[? ?] ?] ?] ?]].
+  eapply type_CongApp ; eassumption.
+Defined.
+
+Lemma type_CongApp' :
+  forall {Σ Γ s1 s2 z1 z2 nx ny np A1 A2 B1 B2 u1 u2 v1 v2 pA pB pu pv},
+    type_glob Σ ->
+    Σ ;;; Γ |-i pA : sHeq (sSort s1) A1 (sSort s2) A2 ->
+    Σ ;;; Γ ,, svass np (sPack A1 A2)
+    |-i pB : sHeq (sSort z1) ((lift 1 1 B1){ 0 := sProjT1 (sRel 0) })
+                 (sSort z2) ((lift 1 1 B2){ 0 := sProjT2 (sRel 0) }) ->
+    Σ ;;; Γ |-i pu : sHeq (sProd nx A1 B1) u1 (sProd ny A2 B2) u2 ->
+    Σ ;;; Γ |-i pv : sHeq A1 v1 A2 v2 ->
+    Σ ;;; Γ ,, svass nx A1 |-i B1 : sSort z1 ->
+    Σ ;;; Γ ,, svass ny A2 |-i B2 : sSort z2 ->
+    Σ ;;; Γ |-i sCongApp B1 B2 pu pA pB pv :
+               sHeq (B1{0 := v1}) (sApp u1 nx A1 B1 v1)
+                    (B2{0 := v2}) (sApp u2 ny A2 B2 v2).
+Proof.
+  intros Σ Γ s1 s2 z1 z2 nx ny np A1 A2 B1 B2 u1 u2 v1 v2 pA pB pu pv
+         hg hpA hpB hpu hpv hB1 hB2.
+  destruct (prod_sorts hg hpA hpB hB1 hB2) as [ss [zz [mm [[e e0] e1]]]].
+  eapply type_CongApp'' ; try eassumption.
+  - eapply heq_sort ; eassumption.
+  - eapply heq_sort ; eassumption.
+  - eapply type_conv' ; eassumption.
+Defined.
+
+Lemma type_CongEq'' :
+  forall {Σ Γ s A1 A2 u1 u2 v1 v2 pA pu pv},
+    type_glob Σ ->
+    Σ ;;; Γ |-i pA : sHeq (sSort s) A1 (sSort s) A2 ->
+    Σ ;;; Γ |-i pu : sHeq A1 u1 A2 u2 ->
+    Σ ;;; Γ |-i pv : sHeq A1 v1 A2 v2 ->
+    Σ ;;; Γ |-i sCongEq pA pu pv :
+               sHeq (sSort s) (sEq A1 u1 v1) (sSort s) (sEq A2 u2 v2).
+Proof.
+  intros Σ Γ s A1 A2 u1 u2 v1 v2 pA pu pv hg hpA hpu hpv.
+  destruct (istype_type hg hpA) as [? iA].
+  destruct (istype_type hg hpu) as [? iu].
+  destruct (istype_type hg hpv) as [? iv].
+  destruct (inversionHeq hg iA) as [? [[[[? ?] ?] ?] ?]].
+  destruct (inversionHeq hg iu) as [? [[[[? ?] ?] ?] ?]].
+  destruct (inversionHeq hg iv) as [? [[[[? ?] ?] ?] ?]].
+  eapply type_CongEq.
+  all: assumption.
+Defined.
+
+Lemma type_CongEq' :
+  forall {Σ Γ s1 s2 A1 A2 u1 u2 v1 v2 pA pu pv},
+    type_glob Σ ->
+    Σ ;;; Γ |-i pA : sHeq (sSort s1) A1 (sSort s2) A2 ->
+    Σ ;;; Γ |-i pu : sHeq A1 u1 A2 u2 ->
+    Σ ;;; Γ |-i pv : sHeq A1 v1 A2 v2 ->
+    Σ ;;; Γ |-i sCongEq pA pu pv
+             : sHeq (sSort s1) (sEq A1 u1 v1)
+                    (sSort s2) (sEq A2 u2 v2).
+Proof.
+  intros Σ Γ s1 s2 A1 A2 u1 u2 v1 v2 pA pu pv hg hpA hpu hpv.
+  destruct (istype_type hg hpA) as [? iA].
+  destruct (istype_type hg hpu) as [? iu].
+  destruct (istype_type hg hpv) as [? iv].
+  destruct (inversionHeq hg iA) as [? [[[[? hs2] ?] hA2] ?]].
+  destruct (inversionHeq hg iu) as [? [[[[? ?] ?] ?] ?]].
+  destruct (inversionHeq hg iv) as [? [[[[? ?] ?] ?] ?]].
+  eapply type_conv'.
+  - assumption.
+  - eapply type_CongEq''.
+    + assumption.
+    + eapply heq_sort ; eassumption.
+    + eassumption.
+    + eassumption.
+  - apply cong_Heq.
+    all: try (apply eq_reflexivity).
+    + eassumption.
+    + apply sorts_in_sort ; assumption.
+    + apply type_Eq ; assumption.
+    + eapply type_conv'.
+      * assumption.
+      * apply type_Eq ; [ apply hA2 | assumption .. ].
+      * eapply sorts_in_sort ; [ apply hs2 | assumption ].
+Defined.
+
+Lemma type_CongRefl'' :
+  forall {Σ Γ s A1 A2 u1 u2 pA pu},
+    type_glob Σ ->
+    Σ ;;; Γ |-i pA : sHeq (sSort s) A1 (sSort s) A2 ->
+    Σ ;;; Γ |-i pu : sHeq A1 u1 A2 u2 ->
+    Σ ;;; Γ |-i sCongRefl pA pu :
+               sHeq (sEq A1 u1 u1) (sRefl A1 u1) (sEq A2 u2 u2) (sRefl A2 u2).
+Proof.
+  intros Σ Γ s A1 A2 u1 u2 pA pu hg hpA hpu.
+  destruct (istype_type hg hpA) as [? iA].
+  destruct (istype_type hg hpu) as [? iu].
+  destruct (inversionHeq hg iA) as [? [[[[? ?] ?] ?] ?]].
+  destruct (inversionHeq hg iu) as [? [[[[? ?] ?] ?] ?]].
+  eapply type_CongRefl.
+  all: eassumption.
+Defined.
+
+Lemma type_CongRefl' :
+  forall {Σ Γ s1 s2 A1 A2 u1 u2 pA pu},
+    type_glob Σ ->
+    Σ ;;; Γ |-i pA : sHeq (sSort s1) A1 (sSort s2) A2 ->
+    Σ ;;; Γ |-i pu : sHeq A1 u1 A2 u2 ->
+    Σ ;;; Γ |-i sCongRefl pA pu :
+               sHeq (sEq A1 u1 u1) (sRefl A1 u1) (sEq A2 u2 u2) (sRefl A2 u2).
+Proof.
+  intros Σ Γ s1 s2 A1 A2 u1 u2 pA pu hg hpA hpu.
+  destruct (istype_type hg hpA) as [? iA].
+  destruct (istype_type hg hpu) as [? iu].
+  destruct (inversionHeq hg iA) as [? [[[[? ?] ?] ?] ?]].
+  destruct (inversionHeq hg iu) as [? [[[[? ?] ?] ?] ?]].
+  eapply type_CongRefl''.
+  - assumption.
+  - eapply heq_sort ; eassumption.
+  - assumption.
+Defined.
+
+Lemma type_EqToHeq' :
+  forall {Σ Γ A u v p},
+    type_glob Σ ->
+    Σ ;;; Γ |-i p : sEq A u v ->
+    Σ ;;; Γ |-i sEqToHeq p : sHeq A u A v.
+Proof.
+  intros Σ Γ A u v p hg h.
+  destruct (istype_type hg h) as [? i].
+  destruct (inversionEq hg i) as [? [[[? ?] ?] ?]].
+  eapply type_EqToHeq ; eassumption.
+Defined.
+
+Lemma type_ProjT1' :
+  forall {Σ Γ A1 A2 p},
+    type_glob Σ ->
+    Σ ;;; Γ |-i p : sPack A1 A2 ->
+    Σ ;;; Γ |-i sProjT1 p : A1.
+Proof.
+  intros Σ Γ A1 A2 p hg hp.
+  destruct (istype_type hg hp) as [? i].
+  destruct (inversionPack hg i) as [s [[? ?] ?]].
+  eapply type_ProjT1 ; [.. | eassumption] ; eassumption.
+Defined.
+
+Lemma type_ProjT2' :
+  forall {Σ Γ A1 A2 p},
+    type_glob Σ ->
+    Σ ;;; Γ |-i p : sPack A1 A2 ->
+    Σ ;;; Γ |-i sProjT2 p : A2.
+Proof.
+  intros Σ Γ A1 A2 p hg hp.
+  destruct (istype_type hg hp) as [? i].
+  destruct (inversionPack hg i) as [s [[? ?] ?]].
+  eapply type_ProjT2 ; [.. | eassumption] ; eassumption.
+Defined.
+
+Lemma type_ProjTe' :
+  forall {Σ Γ A1 A2 p},
+    type_glob Σ ->
+    Σ ;;; Γ |-i p : sPack A1 A2 ->
+    Σ ;;; Γ |-i sProjTe p : sHeq A1 (sProjT1 p) A2 (sProjT2 p).
+Proof.
+  intros Σ Γ A1 A2 p hg hp.
+  destruct (istype_type hg hp) as [? i].
+  destruct (inversionPack hg i) as [s [[? ?] ?]].
+  eapply type_ProjTe ; [.. | eassumption] ; eassumption.
+Defined.
+
+Lemma type_Refl' :
+  forall {Σ Γ A u},
+    type_glob Σ ->
+    Σ ;;; Γ |-i u : A ->
+    Σ ;;; Γ |-i sRefl A u : sEq A u u.
+Proof.
+  intros Σ Γ A u hg h.
+  destruct (istype_type hg h) as [? i].
+  eapply type_Refl ; eassumption.
+Defined.
+
+Lemma type_Transport' :
+  forall {Σ Γ s T1 T2 p t},
+    type_glob Σ ->
+    Σ ;;; Γ |-i p : sEq (sSort s) T1 T2 ->
+    Σ ;;; Γ |-i t : T1 ->
+    Σ ;;; Γ |-i sTransport T1 T2 p t : T2.
+Proof.
+  intros Σ Γ s T1 T2 p t hg hp ht.
+  destruct (istype_type hg hp) as [? i].
+  destruct (inversionEq hg i) as [? [[[? ?] ?] ?]].
+  eapply type_Transport ; eassumption.
+Defined.
+
+Lemma type_HeqTypeEq' :
+  forall {Σ Γ A u B v p s},
+    type_glob Σ ->
+    Σ ;;; Γ |-i p : sHeq A u B v ->
+    Σ ;;; Γ |-i A : sSort s ->
+    Σ ;;; Γ |-i sHeqTypeEq p : sEq (sSort s) A B.
+Proof.
+  intros Σ Γ A u B v p s hg hp hA.
+  destruct (istype_type hg hp) as [? i].
+  destruct (inversionHeq hg i) as [? [[[[? ?] ?] ?] ?]].
+  eapply type_HeqTypeEq ; try eassumption.
+  destruct (uniqueness pi1_ hA).
+  eapply type_conv' ; eassumption.
+Defined.
